Defined Rust-style Iterator

src/Enumeration/Loopers.dfy
@@ -66,7 +66,7 @@ module Loopers {
     }
   }
 
-  trait Enumerator<T> extends Stepper {
+  trait {:termination false} Enumerator<T> extends Stepper {
 
     // Any enumerator that produces one value at a time
     // and provably terminates is equivalent to an enumerator
@@ -237,90 +237,93 @@ module Loopers {
     }
   }
 
-  // class SeqIteratorEnumerator<T(0)> extends Enumerator<T> {
+  class SeqIteratorEnumerator<T(0)> extends Enumerator<T> {
 
-  //   const iter: SeqIterator<T>
-  //   var done: bool
+    const iter: SeqIterator<T>
+    var done: bool
 
-  //   ghost const original: seq<T>
+    ghost const original: seq<T>
 
-  //   constructor(s: seq<T>) 
-  //     ensures Valid() 
-  //     ensures fresh(Repr) 
-  //   {
-  //     iter := new SeqIterator(s);
-  //     original := s;
-  //     enumerated := [];
+    constructor(s: seq<T>) 
+      ensures Valid() 
+      ensures fresh(Repr) 
+    {
+      iter := new SeqIterator(s);
+      original := s;
+      enumerated := [];
       
-  //     new;
+      new;
 
-  //     // Calling MoveNext() right away ensures we only enumerated yielded state.
-  //     // Another version of this adaptor could not do this, and by consequence
-  //     // enumerate the initial state of the iterator as well.
-  //     var more := iter.MoveNext();
-  //     done := !more;
+      // Calling MoveNext() right away ensures we only enumerated yielded state.
+      // Another version of this adaptor could not do this, and by consequence
+      // enumerate the initial state of the iterator as well.
+      var more := iter.MoveNext();
+      done := !more;
       
-  //     Repr := {this, iter} + iter._modifies + iter._reads + iter._new;
-  //   }
+      Repr := {this, iter} + iter._modifies + iter._reads + iter._new;
+    }
 
-  //   predicate Valid() reads this, Repr ensures Valid() ==> this in Repr {
-  //     && this in Repr
-  //     && iter in Repr
-  //     && this !in iter._modifies
-  //     && this !in iter._reads
-  //     && this !in iter._new
-  //     && iter._modifies <= Repr
-  //     && iter._reads <= Repr
-  //     && iter._new <= Repr
-  //     && (!done ==> iter.Valid())
-  //     && iter.elements < iter.s
-  //     && |enumerated| <= |original|
-  //     && enumerated == original[0..|enumerated|]
-  //   }
+    predicate Valid() reads this, Repr ensures Valid() ==> this in Repr {
+      && this in Repr
+      && iter in Repr
+      && this !in iter._modifies
+      && this !in iter._reads
+      && this !in iter._new
+      && iter._modifies <= Repr
+      && iter._reads <= Repr
+      && iter._new <= Repr
+      && (!done ==> iter.Valid())
+      && (!done ==> enumerated + [Current()] == iter.elements)
+      && (done ==> enumerated == iter.elements)
+      && iter.elements < iter.s
+      && |enumerated| <= |original|
+      && enumerated == original[0..|enumerated|]
+    } 
 
-  //   predicate method Done()
-  //     requires Valid()
-  //     reads this, Repr
-  //     decreases Repr, 0
-  //     ensures Decreases() == 0 ==> Done()
-  //     // ensures Done() ==> enumerated == original
-  //   {
-  //     done
-  //   }
+    predicate method Done()
+      requires Valid()
+      reads this, Repr
+      decreases Repr, 0
+      ensures Decreases() == 0 ==> Done()
+      // ensures Done() ==> enumerated == original
+    {
+      done
+    }
 
-  //   method Step()
-  //     requires Valid()
-  //     requires !Done()
-  //     modifies Repr
-  //     decreases Repr
-  //     ensures ValidAndDisjoint()
-  //     ensures Decreases() < old(Decreases())
-  //     ensures enumerated == old(enumerated) + [old(Current())]
-  //   {
-  //     enumerated := enumerated + [Current()];
+    method Step()
+      requires Valid()
+      requires !Done()
+      modifies Repr
+      decreases Repr
+      ensures Valid()
+      ensures Repr <= old(Repr) 
+      ensures Decreases() < old(Decreases())
+      ensures enumerated == old(enumerated) + [old(Current())]
+    {
+      enumerated := enumerated + [Current()];
 
-  //     var more := iter.MoveNext();
-  //     done := !more;
+      var more := iter.MoveNext();
+      done := !more;
 
-  //     Repr := {this, iter} + iter._modifies + iter._reads + iter._new;
-  //   }
+      Repr := {this, iter} + iter._modifies + iter._reads + iter._new;
+    }
 
-  //   function method Current(): T
-  //     reads this, Repr
-  //     requires Valid()
-  //     requires !Done()
-  //   {
-  //     iter.element
-  //   }
+    function method Current(): T
+      reads this, Repr
+      requires Valid()
+      requires !Done()
+    {
+      iter.element
+    }
 
-  //   function Decreases(): nat 
-  //     reads this, Repr 
-  //     requires Valid() 
-  //   {
-  //     assert iter.elements < iter.s;
-  //     (|iter.s| - |iter.elements|) //+ (if done then 0 else 1)
-  //   }
-  // }
+    function Decreases(): nat 
+      reads this, Repr 
+      requires Valid() 
+    {
+      assert iter.elements < iter.s;
+      (|iter.s| - |iter.elements|) //+ (if done then 0 else 1)
+    }
+  }
 
   class ConcatEnumerator<T(0)> extends Enumerator<T> {
 
