src/Enumeration/RustStyle.dfy
@@ -1,0 +1,145 @@
+
+include "../Frames.dfy"
+include "../Wrappers.dfy"
+include "Loopers.dfy"
+
+module RustStyle {
+
+  import opened Frames
+  import opened Wrappers
+  import opened Loopers
+
+  trait RustStyleIterator<T> extends Validatable {
+
+    method Next() returns (res: Option<T>)
+      requires Valid()
+      modifies Repr
+      ensures Valid()
+      ensures Repr <= old(Repr)
+      ensures res.Some? ==> Decreases() < old(Decreases())
+      ensures old(Decreases()) == 0 ==> res.None?
+
+    function Decreases(): nat
+      reads Repr
+      requires Valid()
+  }
+
+  class RustStyleIteratorEnumerator<T> extends Enumerator<T> {
+
+    const iter: RustStyleIterator<T>
+    var next: Option<T>
+
+    ghost var decr: nat
+
+    constructor(iter: RustStyleIterator<T>)
+      requires iter.Valid()
+      modifies iter.Repr
+    {
+      this.iter := iter;
+      new;
+      this.next := iter.Next();
+      Repr := {this} + iter.Repr;
+      if this.next.None? {
+        decr := 0;
+      } else {
+        decr := iter.Decreases() + 1;
+      }
+    }
+
+    predicate Valid() 
+      reads this, Repr 
+      ensures Valid() ==> this in Repr 
+      decreases Repr
+    {
+      && this in Repr
+      && ValidComponent(iter)
+      && decr == (if this.next.None? then 0 else iter.Decreases() + 1)
+    }
+
+    method Step() 
+      requires Valid()
+      requires !Done()
+      modifies Repr
+      decreases Repr
+      ensures Valid()
+      ensures Repr <= old(Repr)
+      ensures Decreases() < old(Decreases())
+      ensures enumerated == old(enumerated) + [old(Current())]
+    {
+      enumerated := enumerated + [Current()];
+      next := iter.Next();
+      if this.next.None? {
+        decr := 0;
+      } else {
+        decr := iter.Decreases() + 1;
+      }
+    }
+
+    function method Current(): T
+      reads this, Repr
+      requires Valid()
+      requires !Done()
+    {
+      next.value
+    }
+
+    function Decreases(): nat
+      reads Repr
+      requires Valid()
+    {
+      decr
+    }
+
+    predicate method Done() 
+      reads Repr
+      requires Valid()
+      decreases Repr, 0
+      ensures Decreases() == 0 ==> Done()
+    {
+      next.None?
+    }
+  }
+
+  class SeqRustStyleIterator extends RustStyleIterator<int> {
+
+    var s: seq<int>
+
+    constructor(s: seq<int>) 
+      ensures Valid()
+    {
+      this.s := s;
+      Repr := {this};
+    }
+
+    predicate Valid() 
+      reads this, Repr 
+      ensures Valid() ==> this in Repr 
+      decreases Repr
+    {
+      && this in Repr
+    }
+
+    method Next() returns (res: Option<int>)
+      requires Valid()
+      modifies Repr
+      ensures Valid()
+      ensures Repr <= old(Repr)
+      ensures res.Some? ==> Decreases() < old(Decreases())
+      ensures old(Decreases()) == 0 ==> res.None?
+    {
+      if |s| > 0 {
+        res := Some(s[0]);
+        s := s[1..];
+      } else {
+        res := None;
+      }
+    }
+
+    function Decreases(): nat
+      reads Repr
+      requires Valid()
+    {
+      |s|
+    }
+  }
+}
